{"cells":[{"cell_type":"markdown","metadata":{"id":"aPUJxdII8yIf"},"source":["# **Ordinary Least Squares (OLS)**\n","**BLUE** : Best Linear Unbiased Estimator (Best means efficient)\n","\n","<br/>\n","\n","## Proof of the OLS formula\n","suppose\n","$\\hat y = \\hat\\alpha + \\hat\\beta x_i$  \n","we should minimize\n","$\\displaystyle S = \\sum_{n=1}^{N}(y_i - \\hat y_i)^2 $\n",", so\n","$\\hat\\alpha$ and $\\hat\\beta$\n","should satisfy\n","$\\displaystyle\\frac{\\partial S}{\\partial \\hat\\alpha} = 0$\n","and\n","$\\displaystyle\\frac{\\partial S}{\\partial \\hat\\beta} = 0$\n","\n","\\begin{gather}\n","\\displaystyle\\frac{\\partial S}{\\partial \\hat\\alpha} = -2\\sum_{i=0}^{N}(y_i-\\hat\\alpha-\\hat\\beta x_i)=0 \\quad \\textrm{(I)}  \\\\\n","\\displaystyle\\frac{\\partial S}{\\partial \\hat\\beta} = -2 \\sum_{i=1}^Nx_i(y_i-\\hat\\alpha-\\hat\\beta x_i)=0\\quad\\textrm{(II)}\n","\\end{gather}  \n","<br/><br/>\n","\n","* Lemma : $\\displaystyle \\sum_{i=1}^N(x_i-\\bar x)(y_i-\\bar y) = \\sum_{i=1}^Ny_i(x_i-\\bar x) = \\sum_{i=1}^N x_i(y_i-\\bar y)$  \n","Proof :\n","\\begin{aligned}\n","\\displaystyle \\sum_{i=1}^N(x_i-\\bar x)(y_i-\\bar y)& = \\sum_{i=1}^Nx_iy_i-\\bar y\\sum_{i=1}^Nx_i - \\bar x\\sum_{i=1}^Ny_i+N\\bar x \\bar y \\\\\n","&= \\sum_{i=1}^Nx_iy_i-N\\bar x \\bar y-N\\bar x \\bar y+N\\bar x \\bar y = \\sum_{i=1}^Nx_iy_i+\\bar x \\sum_{i=1}^N y_i \\\\\n","&= \\sum_{i=1}^Ny_i(x_i-\\bar x)\n","\\end{aligned}\n","and same for $\\displaystyle \\sum_{i=1}^N x_i(y_i-\\bar y)$.  \n","\n","<br/><br/>\n","\n","\\begin{gather}\n","\\textrm{(I)} \\rightarrow \\displaystyle \\sum_{i=1}^Ny_i = \\hat\\alpha\\sum_{i=1}^N1+\\hat\\beta\\sum_{i=1}^Nx_i, \\quad so \\quad\\bar y = \\hat\\alpha + \\hat\\beta\\bar x,\\quad \\hat\\alpha=\\bar y -\\hat\\beta\\bar x\\quad \\textrm{(III)} \\\\  \n","\\textrm{(II)} \\rightarrow \\displaystyle \\sum_{i=1}^Nx_iy_i=\\hat\\alpha\\sum_{i=1}^Nx_i+\\hat\\beta\\sum_{i=1}^Nx_i^2 = (\\bar y -\\hat\\beta\\bar x)N\\bar x +\\hat\\beta\\sum_{i=1}^Nx_i^2 = N\\bar x \\bar y - \\hat\\beta N\\bar x^2 + \\hat\\beta\\sum_{i=1}^Nx_i^2 \\newline\\newline\n","\\displaystyle \\hat\\beta =\\frac{\\sum\\limits_{i=1}^Nx_iy_i-N\\bar x \\bar y}{\\sum\\limits_{i=1}^Nx_i^2-N\\bar x} = \\frac{\\sum\\limits_{i=1}^N(x_iy_i-\\bar x y_i)}{\\sum\\limits_{i=1}^N(x_i^2-\\bar x x_i)} = \\frac{\\sum\\limits_{i=1}^N(x_i-\\bar x)(y_i-\\bar y)}{\\sum\\limits_{i=1}^N(x_i-\\bar x)^2}(\\because lemma)\n","\\end{gather}\n","<br/><br/>\n","\\begin{aligned}\n","\\therefore \\quad \\hat\\beta &= \\frac{Cov(X, Y)}{Var(X)} \\\\\n","\\hat\\alpha &= \\bar y -\\hat\\beta\\bar x\n","\\end{aligned}\n","\n","<br/><br/>\n","\n"]}],"metadata":{"colab":{"authorship_tag":"ABX9TyOuJjfXnf/5rBpFQv2oTfUA","provenance":[{"file_id":"1jKDqFUi0F8jFpEEeaNc_r-6jjIeUwIrx","timestamp":1716452009733}]},"kernelspec":{"display_name":"Python 3","name":"python3"},"language_info":{"name":"python"}},"nbformat":4,"nbformat_minor":0}
